\documentclass{article} 

\usepackage{amsmath,amsthm,amssymb}
\usepackage{enumitem}

%\newtheorem{problem}{Problem} 

%\theoremstyle{definition} 

%\newtheorem*{solution}{Solution} 

\begin{document} \title{Assignment 1} 

\author{Monorina Mukhopadhyay, ID 260364335} 

\date{\today}

\maketitle

\begin{itemize}

\item Problem 2.
\begin{enumerate} [label=\alph*]
%
\item The left side of the equation is: 
    $ \left(X \implies Y \right) \lor \left( X \implies Z \right)$ \\
    $ \equiv ( \lnot X \lor Y ) \lor (\lnot X \lor Z)$  \qquad {Condition Identity}  \\
    $ \equiv ( \lnot X \lor Y \lor \lnot X ) \lor (\lnot X \lor Y \lor Z)$  \qquad {Associative Property} \\
    $ \equiv ( \lnot X \lor Y) \lor ( \lnot X \lor Y \lor Z)$   \qquad {Idempotent Identity} \\
    $ \equiv ( \lnot X \lnot X \lor Y \lor Y) \lor (Z)$   \qquad {Associative Identity} \\
    $ \equiv ( \lnot X \lor Y ) \lor ( Z) $  \qquad {Idempotent Identity} \\
    $ \equiv  \lnot X \lor ( Y \lor Z ) $  \qquad {Associative Identity} \\
    $ \equiv X \implies (Y \lor Z ) $  \qquad {Conditional Identity} \\
        %\ite blah
\item Starting from the left side again:
	$ ( P \iff Q) $
	$ \equiv (P \implies Q ) \land (Q \implies P ) $ \qquad {Biconditional Identity} \\
	$ \equiv (P \implies Q ) \land (\lnot Q \lor P) $ \qquad {Conditional Identity} \\
	$ \equiv (P \implies Q ) \land (\lnot (\lnot P) \lor \lnot Q ) $ \qquad {Commutative and Double Negative Properties} \\
	$ \equiv (P \implies Q ) \land (\lnot P \implies \lnot Q) $ \qquad {Conditional Identity} \\
\item Blah



\end{enumerate}
\end{itemize}
\end{document}